Veir/Parser/MlirParser.lean
@@ -201,7 +201,7 @@ partial def parseOptionalOp (ip : Option InsertPoint) : MlirParserM (Option Oper
 
   /- Create the operation. -/
   let opId := operationNameToOpId opName
-  let some (ctx, op) := Rewriter.createOp (← getContext) opId outputTypes operands regions 0 ip (by sorry) (by sorry) (by sorry) (by sorry)
+  let some (ctx, op) := Rewriter.createOp (← getContext) opId outputTypes operands #[] regions 0 ip (by sorry) (by sorry) (by sorry) (by sorry) (by sorry)
       | throw "internal error: failed to create operation"
 
   /- Update the parser context. -/
